\documentclass{article}
\usepackage[a4paper, total={6.5in, 8in}]{geometry}
\usepackage[utf8]{inputenc}
\usepackage[T1]{fontenc}
\usepackage{hyperref}
\usepackage{float}
\usepackage{amsmath}
\usepackage{booktabs}
\usepackage{mathtools}
\usepackage{amsfonts}
\usepackage{amssymb}
\usepackage{graphicx}
\usepackage{cases}
\usepackage{parskip}
\title{Some random problem}
\date{}
\begin{document}

Let \(E\) be the arithmetic mean of \(a_i\): \(E = \frac{1}{n}\sum_{i=1}^{n} a_i\). Also let 
\[
    V = \frac{1}{n}\sum_{i=1}^{n} (a_{i}-E)^2 = \frac{1}{n}\sum_{i=1}^{n} a_i^2 - \frac{2}{n} \sum_{i=1}^{n} a_i E + n \cdot \frac{E^2}{n} = \frac{1}{n} \sum_{i=1}^{n} a_i^2 + E(E-\frac{2}{n}\sum_{i=1}^{n} a_i) = \frac{1}{n}\sum_{i=1}^{n} a_i^2 - E^2.
\] 
Let's divide initial inequality by \(n^2\) and substitute the above notation:
\[
    \frac{1}{n}\sum_{i\in A}^{n} a_i^2 + 4 \Bigl( \frac{\sum\limits_{i=1}^{n} a_i}{n} \Bigr) ^2 \leq 4 = \frac{4}{n} \sum_{i=1}^{n} a_i^2
\]
It's sufficient to prove the following inequality:
\[
  \frac{1}{n}\sum_{i\in A}^{n} \frac{a_i^2}{2} \leq V 
\]

From inequality between quadratic and arithmetic mean we know that \( \sqrt{\frac{\sum_{i=1}^{n} a_i^2}{n} }\geq  \frac{\sum_{i=1}^{n} a_i}{n} \implies \sum_{i=1}^{n} a_i \leq n \). 
Moreover, since \(a \geq 2 \), then \(a-1 \geq \frac{a}{2}\).  
However, 
\[
    V = \frac{1}{n}\sum_{i=1}^{n} (a_i - E)^2 \geq \frac{1}{n}\sum_{i\in A}^{n} (a_{i}-E)^2 \geq \frac{1}{n}\sum_{i\in A}^{n} (a_i -1)^2 \geq \frac{1}{n}\sum_{i\in A}^{n} \bigl(\frac{a_i}{2} \bigr) ^2, 
\]
which ends the proof.


\end{document}

